Second draft of proof; recursively transforms call and invocation arguments

proof_of_soundness/.CoqMakefile.d
@@ -1,15 +1,18 @@
 ConfigVars.vo ConfigVars.glob ConfigVars.v.beautified ConfigVars.required_vo: ConfigVars.v Syntax.vo
 ConfigVars.vio: ConfigVars.v Syntax.vio
 ConfigVars.vos ConfigVars.vok ConfigVars.required_vos: ConfigVars.v Syntax.vos
-EvalRules.vo EvalRules.glob EvalRules.v.beautified EvalRules.required_vo: EvalRules.v Syntax.vo ConfigVars.vo
-EvalRules.vio: EvalRules.v Syntax.vio ConfigVars.vio
-EvalRules.vos EvalRules.vok EvalRules.required_vos: EvalRules.v Syntax.vos ConfigVars.vos
+EvalRules.vo EvalRules.glob EvalRules.v.beautified EvalRules.required_vo: EvalRules.v ConfigVars.vo Syntax.vo
+EvalRules.vio: EvalRules.v ConfigVars.vio Syntax.vio
+EvalRules.vos EvalRules.vok EvalRules.required_vos: EvalRules.v ConfigVars.vos Syntax.vos
+MapTheorems.vo MapTheorems.glob MapTheorems.v.beautified MapTheorems.required_vo: MapTheorems.v ConfigVars.vo
+MapTheorems.vio: MapTheorems.v ConfigVars.vio
+MapTheorems.vos MapTheorems.vok MapTheorems.required_vos: MapTheorems.v ConfigVars.vos
 Syntax.vo Syntax.glob Syntax.v.beautified Syntax.required_vo: Syntax.v 
 Syntax.vio: Syntax.v 
 Syntax.vos Syntax.vok Syntax.required_vos: Syntax.v 
-Theorems.vo Theorems.glob Theorems.v.beautified Theorems.required_vo: Theorems.v Syntax.vo ConfigVars.vo EvalRules.vo Transformations.vo
-Theorems.vio: Theorems.v Syntax.vio ConfigVars.vio EvalRules.vio Transformations.vio
-Theorems.vos Theorems.vok Theorems.required_vos: Theorems.v Syntax.vos ConfigVars.vos EvalRules.vos Transformations.vos
+Theorems.vo Theorems.glob Theorems.v.beautified Theorems.required_vo: Theorems.v Syntax.vo ConfigVars.vo MapTheorems.vo EvalRules.vo Transformations.vo
+Theorems.vio: Theorems.v Syntax.vio ConfigVars.vio MapTheorems.vio EvalRules.vio Transformations.vio
+Theorems.vos Theorems.vok Theorems.required_vos: Theorems.v Syntax.vos ConfigVars.vos MapTheorems.vos EvalRules.vos Transformations.vos
 Transformations.vo Transformations.glob Transformations.v.beautified Transformations.required_vo: Transformations.v Syntax.vo ConfigVars.vo EvalRules.vo
 Transformations.vio: Transformations.v Syntax.vio ConfigVars.vio EvalRules.vio
 Transformations.vos Transformations.vok Transformations.required_vos: Transformations.v Syntax.vos ConfigVars.vos EvalRules.vos
