proof_of_soundness/EvalRules.v
@@ -1,5 +1,6 @@
 Require Import
   Coq.Lists.List
+  Coq.Logic.Classical_Prop
   Coq.Strings.String
   Coq.ZArith.ZArith.
 
@@ -7,12 +8,6 @@ From Cpp2C Require Import
   ConfigVars
   Syntax.
 
-
-Theorem demorgan : forall A B,
-  ~ (A \/ B) <-> ~A /\ ~B.
-Proof.
-  intros. tauto.
-Qed.
 
 (* Macro substitution.
    Check this for details on nested calls to macros:
@@ -44,6 +39,19 @@ Fixpoint msub
   (* FIXME: This doesn't match the actual semantics of macro expansion
             See the Google Doc *)
   | CallOrInvocation x es => CallOrInvocation x es
+end.
+
+
+Fixpoint fsub
+  (p : string) (e : expr) (fexpr : expr) : expr :=
+  match fexpr with
+   | Num z => Num z
+   | Var x => if String.eqb p x then e else Var x
+   | ParenExpr e0 => ParenExpr (fsub p e e0)
+   | UnExpr uo e0 => UnExpr uo (fsub p e e0)
+   | BinExpr bo e1 e2 => BinExpr bo (fsub p e e1) (fsub p e e2)
+   | Assign x e0 => Assign x e0
+   | CallOrInvocation x es => CallOrInvocation x es
 end.
 
 
@@ -92,19 +100,111 @@ Proof.
   split; induction e; intros; simpl in *;
   try discriminate; try (apply IHe; apply H);
   try apply I; try contradiction; try reflexivity; try auto.
-  - rewrite Bool.orb_false_iff in H. apply demorgan. split.
+  - rewrite Bool.orb_false_iff in H. apply Classical_Prop.and_not_or. split.
     + apply IHe1. apply H.
     + apply IHe2. apply H.
-  - apply demorgan in H. apply Bool.orb_false_iff. split.
+  - apply Classical_Prop.not_or_and in H. apply Bool.orb_false_iff. split.
     + apply IHe1. apply H.
     + apply IHe2. apply H.
 Qed.
+
+
+Inductive StepExpr :
+  store -> environment -> environment ->
+  function_table -> macro_table ->
+  expr ->
+  expr -> store -> Prop :=
+  (* In small step semantics we elide the rules for constants *)
+  
+  (* Variable lookup *)
+  | Step_VarLocal : forall S E G F M x l z,
+    StringMap.MapsTo x l E ->
+    NatMap.MapsTo l z S ->
+    StepExpr S E G F M (Var x) (Num z) S
+  | Step_VarGlobal : forall S E G F M x l z,
+    ~ StringMap.In x E->
+    StringMap.MapsTo x l G ->
+    NatMap.MapsTo l z S ->
+    StepExpr S E G F M (Var x) (Num z) S
+  (* Parenthesized expressions *)
+  
+  | Step_ParenExprConst : forall S E G F M z,
+    StepExpr S E G F M (ParenExpr (Num z)) (Num z) S
+  | Step_ParenExpr1 : forall S E G F M e0 e0' S',
+    StepExpr S E G F M e0 e0' S' ->
+    StepExpr S E G F M (ParenExpr e0) (ParenExpr e0') S'
+  
+  (* Unary expressions *)
+  | Step_UnExprConst : forall S E G F M uo z,
+    StepExpr S E G F M (UnExpr uo (Num z)) (Num (unop_to_op uo z)) S
+  | Step_UnExpr1 : forall S E G F M uo e0 e0' S',
+    StepExpr S E G F M e0 e0' S' ->
+    StepExpr S E G F M (UnExpr uo e0) (UnExpr uo e0') S'
+  
+  (* Binary expressions *)
+  | Step_BinExprConst : forall S E G F M bo z1 z2,
+    StepExpr S E G F M (BinExpr bo (Num z1) (Num z2)) (Num (binop_to_op bo z1 z2)) S
+  | Step_BinExpr1 : forall S E G F M bo e1 e2 e1' S',
+    StepExpr S E G F M e1 e1' S' ->
+    StepExpr S E G F M (BinExpr bo e1 e2) (BinExpr bo e1' e2) S'
+  | Step_BinExpr2 : forall S E G F M bo z1 e2 e2' S',
+    StepExpr S E G F M e2 e2' S' ->
+    StepExpr S E G F M (BinExpr bo (Num z1) e2) (BinExpr bo (Num z1) e2') S'
+  
+  (* Assignments *)
+  | Step_AssignLocalConst : forall S E G F M l x z S',
+    StringMap.MapsTo x l E ->
+    NatMap.Equal S' (NatMapProperties.update S (NatMap.add l z (NatMap.empty Z))) ->
+    StepExpr S E G F M (Assign x (Num z)) (Num z) S'
+  | Step_AssignGlobalConst : forall S E G F M l x z S',
+    ~ StringMap.In x E ->
+    StringMap.MapsTo x l G ->
+    NatMap.Equal S' (NatMapProperties.update S (NatMap.add l z (NatMap.empty Z))) ->
+    StepExpr S E G F M (Assign x (Num z)) (Num z) S'
+  | Step_Assign1 : forall S E G F M x e0 e0' S',
+    StepExpr S E G F M e0 e0' S' ->
+    StepExpr S E G F M (Assign x e0) (Assign x e0') S'
+  
+  
+  (*  TODO: Define small step semantics for
+      function calls and macro invocations *)
+      
+      
+  | Step_FunctionCall : forall S E G F M x params fstmt fexpr es fexpr' S',
+    ~ StringMap.In x M ->
+    StringMap.MapsTo x (params, fstmt, fexpr) F ->
+    StepArgs S E G F M fexpr params es fexpr' S' ->
+    StepExpr S E G F M (CallOrInvocation x es) fexpr' S'
+
+with StepStmt :
+  store -> environment -> environment ->
+  function_table -> macro_table ->
+  stmt -> stmt -> store -> Prop :=
+
+with StepArgs : 
+  store -> environment -> environment ->
+  function_table -> macro_table ->
+  expr -> list string -> list expr ->
+  expr ->
+  store -> Prop :=
+  
+  | Step_ArgsNil : forall S E G F M fexpr,
+    StepArgs S E G F M fexpr nil nil fexpr S
+  
+  | Step_ArgsConsConst : forall S E G F M fexpr fexpr' z p ps es S',
+    StepArgs S E G F M (fsub p (Num z) fexpr) ps es fexpr' S' ->
+    StepArgs S E G F M fexpr (p::ps) ((Num z)::es) fexpr' S'
+  
+  | Step_ArgsConsExpr : forall S E G F M e' S' fexpr fexpr' p ps e es,
+    StepExpr S E G F M e e' S' ->
+    StepArgs S E G F M fexpr (p::ps) (e'::es) fexpr' S' ->
+    StepArgs S E G F M fexpr (p::ps) (e::es) fexpr' S'.
 
 (* Right now, a term that fails to evaluate will simply get "stuck";
    i.e. it will fail to be reduced further.
    We do not provide any error messages, but I think we could add
    this later using a sum type. *)
-Inductive ExprEval:
+Inductive EvalExpr:
   store -> environment -> environment ->
   function_table -> macro_table ->
   expr ->
@@ -112,35 +212,35 @@ Inductive ExprEval:
   (* Numerals evaluate to their integer representation and do not
      change the store *)
   | E_Num : forall S E G F M z,
-    ExprEval S E G F M (Num z) z S
+    EvalExpr S E G F M (Num z) z S
   (* Variable lookup occurs iff a macro parameter is not found. *)
   | E_LocalVar : forall S E G F M x l v,
     StringMap.MapsTo x l E ->
     NatMap.MapsTo l v S ->
-    ExprEval S E G F M (Var x) v S
+    EvalExpr S E G F M (Var x) v S
   (* Local variables shadow global variables, so only if a local
      variable lookup fails do we check the global environment. *)
   | E_GlobalVar : forall S E G F M x l v,
     ~ StringMap.In x E->
     StringMap.MapsTo x l G ->
     NatMap.MapsTo l v S ->
-    ExprEval S E G F M (Var x) v S
+    EvalExpr S E G F M (Var x) v S
   (* Parenthesized expressions evaluate to themselves. *)
   | E_ParenExpr : forall S E G F M e0 v S',
-    ExprEval S E G F M e0 v S' ->
-    ExprEval S E G F M (ParenExpr e0) v S'
+    EvalExpr S E G F M e0 v S' ->
+    EvalExpr S E G F M (ParenExpr e0) v S'
   (* Unary expressions *)
   | E_UnExpr : forall S E G F M S' uo e0 v,
-    ExprEval S E G F M e0 v S' ->
-    ExprEval S E G F M (UnExpr uo e0) ((unop_to_op uo) v) S'
+    EvalExpr S E G F M e0 v S' ->
+    EvalExpr S E G F M (UnExpr uo e0) ((unop_to_op uo) v) S'
   (* Binary expressions. Left operands are evaluated first. *)
   (* NOTE: Evaluation rules do not handle operator precedence.
      The parser must use a concrete syntax to generate a parse tree
      with the appropriate precedence levels in it. *)
   | E_BinExpr : forall S E G F M bo e1 e2 v1 v2 S' S'',
-    ExprEval S E G F M e1 v1 S' ->
-    ExprEval S' E G F M e2 v2 S'' ->
-    ExprEval S E G F M (BinExpr bo e1 e2) ((binop_to_op bo) v1 v2) S''
+    EvalExpr S E G F M e1 v1 S' ->
+    EvalExpr S' E G F M e2 v2 S'' ->
+    EvalExpr S E G F M (BinExpr bo e1 e2) ((binop_to_op bo) v1 v2) S''
   (* Variable assignments update the store by adding a new L-value to
      R-value mapping or by overriding an existing one.
      The R-value is returned along with the updated state.
@@ -150,16 +250,16 @@ Inductive ExprEval:
   (* Local variable assignment overrides global variable assignment. *)
   | E_Assign_Local : forall S E G F M l x e0 v S' S'',
     StringMap.MapsTo x l E ->
-    ExprEval S E G F M e0 v S' ->
+    EvalExpr S E G F M e0 v S' ->
     S'' = NatMapProperties.update S (NatMap.add l v (NatMap.empty Z)) ->
-    ExprEval S E G F M (Assign x e0) v S''
+    EvalExpr S E G F M (Assign x e0) v S''
   (* Global variable assignment *)
   | E_Assign_Global : forall S E G F M l x e0 v S' S'',
     ~ StringMap.In x E ->
     StringMap.MapsTo x l G ->
-    ExprEval S E G F M e0 v S' ->
+    EvalExpr S E G F M e0 v S' ->
     S'' = NatMapProperties.update S (NatMap.add l v (NatMap.empty Z)) ->
-    ExprEval S E G F M (Assign x e0) v S''
+    EvalExpr S E G F M (Assign x e0) v S''
   (* For function calls, we perform the following steps:
      1) Evaluate arguments
      2) Map parameters to arguments in function local environment,
@@ -171,7 +271,7 @@ Inductive ExprEval:
      5) Return the return value and store *)
   | E_FunctionCall:
     forall S E G F M x es params fstmt fexpr ls
-           Sargs S' S'' S''' Ef S'''' S''''' v vs,
+           Ef Sargs S' S'' S''' S'''' S''''' v vs,
     (* TODO: Things to consider :
        - Should all functions have unique names?
     *)
@@ -193,13 +293,13 @@ Inductive ExprEval:
     (* Combine the argument store into the original store *)
     NatMap.Equal S'' (NatMapProperties.update S' Sargs) ->
     (* Evaluate the function's body *)
-    StmtEval S'' Ef G F M fstmt S''' ->
-    ExprEval S''' Ef G F M fexpr v S'''' ->
+    EvalStmt S'' Ef G F M fstmt S''' ->
+    EvalExpr S''' Ef G F M fexpr v S'''' ->
     (* Only keep in the store the L-value mappings that were there when
        the function was called; i.e., remove from the store all mappings
        whose L-value is in Ef/Sargs. *)
     NatMap.Equal S''''' (NatMapProperties.restrict S'''' S) ->
-    ExprEval S E G F M (CallOrInvocation x es) v S'''''
+    EvalExpr S E G F M (CallOrInvocation x es) v S'''''
   (* Macro invocation *)
   | E_MacroInvocation :
     forall S E G F M x params es mexpr M' MP ef S' v,
@@ -219,8 +319,8 @@ Inductive ExprEval:
     (* Create the MP for evaluating the macro expression in *)
     MP = combine params es ->
     ef = msub MP mexpr ->
-    ExprEval S E G F M' ef v S' ->
-    ExprEval S E G F M (CallOrInvocation x es) v S'
+    EvalExpr S E G F M' ef v S' ->
+    EvalExpr S E G F M (CallOrInvocation x es) v S'
 with EvalArgs :
   store -> environment -> environment -> function_table -> macro_table ->
   list expr -> list Z -> store ->
@@ -231,16 +331,16 @@ with EvalArgs :
   (* There are arguments left to evaluate *)
   | EvalArgs_cons : forall Sprev Ecaller G F M e v Snext es vs Sfinal,
     (* Evaluate the first expression using the caller's *)
-    ExprEval Sprev Ecaller G F M e v Snext ->
+    EvalExpr Sprev Ecaller G F M e v Snext ->
     (* Evaluate the remaining expressions *)
     EvalArgs Snext Ecaller G F M es vs Sfinal ->
     (* Return the final environment *)
     EvalArgs Sprev Ecaller G F M (e::es) (v::vs) Sfinal
-with StmtEval :
+with EvalStmt :
   store -> environment -> environment ->
   function_table -> macro_table ->
   stmt ->
   store -> Prop :=
   (* A skip statement does not change the state *)
   | E_Skip : forall S E G F M,
-    StmtEval S E G F M Skip S.
+    EvalStmt S E G F M Skip S.
