proof_of_soundness/Transformations.v
@@ -28,12 +28,18 @@ Inductive TransformExpr :
     TransformExpr M F e0 F' e0' ->
     TransformExpr M F (UnExpr uo e0) F' (UnExpr uo e0')
   
-  | Transform_BinExpr : forall M F e1 e2 F' F'' e1' e2' bo,
+  | Transform_BinExpr : forall M F e1 e2 F1result F2result e1' e2' bo F' F'',
+  
+    (* Transform the left operand *)
+    StringMapProperties.Disjoint F F1result ->
+    F' = StringMapProperties.update F F1result ->
     TransformExpr M F e1 F' e1' ->
-    TransformExpr M F e2 F'' e2' ->
-    (* If an expression is evaluable under F', then it should be evaluable under F'' *)
-    (* There may be a better way to prove this, but I can't figure out how to do it yet *)
-    (forall S E G v S', ExprEval S E G F' M e1' v S' -> ExprEval S E G F'' M e1' v S') ->
+  
+    (* Transform the right operand *)
+    StringMapProperties.Disjoint F' F2result ->
+    F'' = StringMapProperties.update F' F2result ->
+    TransformExpr M F' e2 F'' e2' ->
+  
     TransformExpr M F (BinExpr bo e1 e2) F'' (BinExpr bo e1' e2')
   
   | Transform_Assign : forall M F x e F' e',
@@ -42,89 +48,105 @@ Inductive TransformExpr :
 
   | Transform_FunctionCall :
     forall   F M x es F' F'' F''' F'''' es'
-             params fstmt fexpr fstmt' fexpr',
+             params fstmt fexpr fstmt' fexpr'
+             Fargsresult Fstmtresult Fexprresult fname,
     (* Macros shadow functions, so to determine if what we are calling is a function
        it suffices just to check that its name is not in the macro table and is in
        the function table *)
     ~ StringMap.In x M ->
     StringMap.MapsTo x (params, fstmt, fexpr) F ->
     
-    (* There is only one mapping for x in the original function table *)
-    (forall params0 fstmt0 fexpr0 params1 fstmt1 fexpr1,
-      StringMap.MapsTo x (params0, fstmt0, fexpr0) F ->
-      (params0, fstmt0, fexpr0) = (params1, fstmt1, fexpr1)) ->
-    
-    (* Transform function arguments first *)
+    (* Transform function arguments *)
+    StringMapProperties.Disjoint F Fargsresult ->
+    F' = StringMapProperties.update F Fargsresult ->
     TransformArgs M F es F' es' ->
+    
+    (* Transform function statement *)
+    StringMapProperties.Disjoint F' Fstmtresult ->
+    F'' = StringMapProperties.update F' Fstmtresult ->
     TransformStmt M F' fstmt F'' fstmt' ->
+    
+    (* Transform function return expression *)
+    StringMapProperties.Disjoint F'' Fexprresult ->
+    F''' = StringMapProperties.update F'' Fexprresult ->
     TransformExpr M F'' fexpr F''' fexpr' ->
-    StringMap.Equal F'''' (StringMap.add x (params, fstmt', fexpr') F''') ->
-    TransformExpr M F (CallOrInvocation x es) F'''' (CallOrInvocation x es')
+
+    (* Add the transformed function back to the function table under a new name *)
+    ~ StringMap.In fname M ->
+    ~ StringMap.In fname F''' ->
+    F'''' = StringMap.add fname (params, fstmt', fexpr') F''' ->
+
+    TransformExpr M F (CallOrInvocation x es) F'''' (CallOrInvocation fname es')
     
   | Transform_SideEffectFreeMacro :
-    forall  F M x es F' F'' es' params mexpr fname
-  
-          (S : store) (E : environment) (G : environment)
-          (vs : list Z) (ls : list nat) (v : Z) (Ef : environment)
-          Sargs S' S'' S''' S'''' S''''',
+    forall  F M x es F' F'' Fes' es' params mexpr fname
+            (vs : list Z) (ls : list nat) (v : Z) (Ef : environment)
+            (Sargs : store) (S' : store) (S'' : store) (S''' : store)
+            (S'''' : store) (S''''' : store),
     (* Again, macros shadow functions, so we just have to check if the callee's name
        is in the macro table to determine if it is a macro. *)
     
     StringMap.MapsTo x (params, mexpr) M ->
     
-    (* There is only one mapping for x in the macro table *)
-    (forall params0 mexpr0 params1 mexpr1,
-      StringMap.MapsTo x (params0, mexpr0) M ->
-      (params0, mexpr0) = (params1, mexpr1) ) ->
-    
     (* The macro does not have side-effects *)
     ~ ExprHasSideEffects mexpr ->
     Forall (fun e => ~ ExprHasSideEffects e) es ->
     
-    (* Transform macro arguments first *)
+    (* Transform macro arguments *)
+    StringMapProperties.Disjoint F Fes' ->
+    F' = StringMapProperties.update F Fes' ->
     TransformArgs M F es F' es' ->
     
     (* Add the transformed function definition to the function table *)
+    ~ StringMap.In fname M ->
     ~ StringMap.In fname F' ->
-    StringMap.Equal F'' (StringMap.add fname (params, Skip, mexpr) F') ->
-    
-    
+    F'' = StringMap.add fname (params, Skip, mexpr) F' ->
     
     
     (* We need to manually add all the premises for function calls that we can't
        intuit from the proof context alone, because macro invocation just doesn't do
        certain things that function calls do, such as evaluating arguments in an
        eager manner *)
-    (* These premises are currently too lenient though; we should only use the original
-       F in these and prove that they will still hold under F'' *)
-       ~ StringMap.In fname M ->
-      (* StringMap.MapsTo x (params, fstmt, fexpr) F /\ *) (* We can prove this *)
-      (* NoDup params /\ *) (* This is given from the macro invocation *)
-      EvalArgs S E G F M es vs S' ->
-      StringMap.Equal Ef (StringMapProperties.of_list (combine params ls)) ->
-      NatMap.Equal Sargs (NatMapProperties.of_list (combine ls vs)) ->
-      NatMapProperties.Disjoint S' Sargs ->
-      NatMap.Equal S'' (NatMapProperties.update S' Sargs) ->
-      StmtEval S'' Ef G F M Skip S''' ->
-      ExprEval S''' Ef G F M mexpr v S'''' ->
-      NatMap.Equal S''''' (NatMapProperties.restrict S'''' S) ->
     
+    (* TODO: Fix these premises *)
+
+    (forall (S : store) (E : environment) (G : environment)
+            (vs : list Z) (ls : list nat) (v : Z) (Ef : environment)
+            (Sargs : store) (S' : store) (S'' : store) (S''' : store)
+            (S'''' : store) (S''''' : store),
+
+      EvalArgs S E G F M es vs S' /\
+      StringMap.Equal Ef (StringMapProperties.of_list (combine params ls)) /\
+      NatMap.Equal Sargs (NatMapProperties.of_list (combine ls vs)) /\
+      NatMapProperties.Disjoint S' Sargs /\
+      NatMap.Equal S'' (NatMapProperties.update S' Sargs) /\
+      EvalStmt S'' Ef G F M Skip S''' /\
+      
+      EvalExpr S''' Ef G F M mexpr v S'''' /\
+      NatMap.Equal S''''' (NatMapProperties.restrict S'''' S)) ->
     
-    TransformExpr M F (CallOrInvocation x es) F'' (CallOrInvocation fname es)
+    TransformExpr M F (CallOrInvocation x es) F'' (CallOrInvocation fname es')
 with TransformArgs :
   macro_table -> function_table -> list expr ->
   function_table -> list expr -> Prop :=
   
   (* End of arguments *)
-  | TransformArgs_Nil : forall M F es,
-    TransformArgs M F nil F es
+  | TransformArgs_Nil : forall M F,
+    TransformArgs M F nil F nil
   
   (* There are arguments left to transform *)
-  | TransformArgs_Cons : forall M F e es F' F'' e' es',
+  | TransformArgs_Cons : forall M F e es F' F'' Fe' Fes' e' es',
     (* Transform the first expression *)
+    StringMapProperties.Disjoint F Fe' ->
+    F' = StringMapProperties.update F Fe' ->
     TransformExpr M F e F' e' ->
+    
     (* Transform the remaining expressions *)
+    StringMapProperties.Disjoint F' Fes' ->
+    F'' = StringMapProperties.update F' Fes' ->
     TransformArgs M F' es F'' es' ->
+    
+    
     TransformArgs M F (e::es) F'' (e'::es')
 with TransformStmt :
   macro_table -> function_table -> stmt ->
@@ -135,11 +157,104 @@ with TransformStmt :
 
 
 
+Inductive StepTransformExpr :
+  macro_table -> function_table -> expr ->
+  function_table -> expr -> Prop :=
+  
+  | StepTransform_Var : forall M F x,
+    StepTransformExpr M F (Var x) F (Var x)
+  
+  | StepTransform_ParenExpr : forall M F e0 F' e0',
+    StepTransformExpr M F e0 F' e0' ->
+    StepTransformExpr M F (ParenExpr e0) F' (ParenExpr e0')
+  
+  | StepTransform_UnExpr : forall M F e0 F' e0' uo,
+    StepTransformExpr M F e0 F' e0' ->
+    StepTransformExpr M F (UnExpr uo e0) F' (UnExpr uo e0')
+  
+  
+  | StepTransform_BinExprConst : forall M F bo z1 z2,
+    StepTransformExpr M F (BinExpr bo (Num z1) (Num z2)) F (BinExpr bo (Num z1) (Num z2))
+  | StepTransform_BinExpr1 : forall M F bo e1 e2 e1' F',
+    StepTransformExpr M F e1 F' e1' ->
+    StepTransformExpr M F (BinExpr bo e1 e2) F' (BinExpr bo e1' e2)
+  | StepTransform_BinExpr2 : forall M F bo z1 e2 e2' F',
+    StepTransformExpr M F e2 F' e2' ->
+    StepTransformExpr M F (BinExpr bo (Num z1) e2) F' (BinExpr bo (Num z1) e2')
+  
+  | StepTransform_Assign : forall M F x e0 F' e0',
+    StepTransformExpr M F e0 F' e0' ->
+    StepTransformExpr M F (Assign x e0) F' (Assign x e0')
+  
+  | StepTransform_Call : forall M F x es F' es',
+    StepTransformArgs M F es F' es' ->
+    StepTransformExpr M F (CallOrInvocation x es) F (CallOrInvocation x es')
+  
+with StepTransformStmt :
+  macro_table -> function_table -> stmt ->
+  function_table -> stmt -> Prop :=
+  
+  | StepTransformSkip : forall M F,
+    StepTransformStmt M F Skip F Skip
+  
+with StepTransformArgs :
+  macro_table -> function_table -> list expr ->
+  function_table -> list expr -> Prop :=
+  | StepTransformArgsNil : forall M F,
+    StepTransformArgs M F nil F nil
+  | StepTransformArgsCons : forall M F e es F' F'' e' es',
+    StepTransformExpr M F e F' e' ->
+    StepTransformArgs M F' es F'' es' ->
+    StepTransformArgs M F (e::es) F'' (e'::es').
 
 
+Scheme StepTransformExpr_mut := Induction for StepTransformExpr Sort Prop
+with StepTransformArgs_mut := Induction for StepTransformArgs Sort Prop.
 
 
+Lemma StepTransformExpr_StepExpr_StepExpr : forall M F e0 F' e1,
+  StepTransformExpr M F e0 F' e1 ->
+  forall S E G e' S',
+    StepExpr S E G F M e0 e' S' ->
+    StepExpr S E G F' M e1 e' S'.
+Proof.
 
+  intros.
+  apply (
+    StepTransformExpr_mut
+      (fun M F e0 F' e1 (h : StepTransformExpr M F e0 F' e1) =>
+        forall S E G e' S',
+          StepExpr S E G F M e0 e' S' ->
+          StepExpr S E G F M e1 e' S')
+      (fun M F es F' es' (h : StepTransformArgs M F es F' es') =>
+        forall S E G F M S' fexpr fexpr' ps,
+          StepArgs S E G F M fexpr ps es fexpr' S' ->
+          StepArgs S E G F M fexpr ps es' fexpr' S')
+    ) with e0 F; auto.
+  - intros. inversion H2; subst.
+    + inversion s.
+    + apply Step_ParenExpr1. apply H1. auto.
+  - intros. inversion H2; subst.
+    + inversion s; subst.
+    + constructor. apply H1. auto.
+  - intros. inversion H2; subst.
+    + inversion s; subst.
+    + apply Step_BinExpr1; auto.
+    + inversion s.
+  - intros. inversion H2; subst.
+    + inversion s.
+    + inversion H13.
+    + apply Step_BinExpr2. apply H1. auto.
+  - intros. inversion H2; subst.
+    + inversion s.
+    + inversion s.
+    + apply Step_Assign1. apply H1. auto.
+  - intros. inversion H2; subst.
+    apply Step_FunctionCall with params fstmt fexpr; auto.
+  - intros. admit.
+  - admit.
+  - admit.
+Abort.
 
 
 
