proof_of_soundness/MapTheorems.v
@@ -1,0 +1,148 @@
+Require Import
+  Coq.FSets.FMapList
+  Coq.ZArith.ZArith.
+  
+From Cpp2C Require Import
+  ConfigVars.
+
+
+
+Lemma NatMap_Empty_empty : forall (t : Type) (m : NatMap.t t),
+  NatMap.Empty (elt:=_) m ->
+  NatMap.Equal m (NatMap.empty _).
+Proof.
+  intros.
+  unfold NatMap.Empty in H.
+  apply NatMapProperties.elements_Empty in H.
+  unfold NatMap.Equal. intros.
+  rewrite NatMapFacts.elements_o. rewrite H. simpl.
+  rewrite NatMapFacts.empty_o. reflexivity.
+Qed.
+
+
+Lemma StringMap_Empty_empty : forall (t : Type) (m : StringMap.t t),
+  StringMap.Empty (elt:=_) m ->
+  StringMap.Equal m (StringMap.empty _).
+Proof.
+  intros.
+  unfold StringMap.Empty in H.
+  apply StringMapProperties.elements_Empty in H.
+  unfold StringMap.Equal. intros.
+  rewrite StringMapFacts.elements_o. rewrite H. simpl.
+  rewrite StringMapFacts.empty_o. reflexivity.
+Qed.
+
+
+Lemma NatMap_restrict_refl: forall (S : store),
+  NatMap.Equal S (NatMapProperties.restrict S S).
+Proof.
+  intros. rewrite NatMapFacts.Equal_mapsto_iff.
+  intros. rewrite NatMapProperties.restrict_mapsto_iff.
+  split; intros.
+  - (* -> *)
+    split.
+    + apply H.
+    + apply NatMapFacts.find_mapsto_iff in H.
+      apply NatMapFacts.in_find_iff. unfold not.
+      intros. rewrite H0 in H. discriminate H.
+  - (* <- *)
+    apply H.
+Qed.
+
+
+Lemma NatMap_mapsto_in: forall (S : store) l v,
+  NatMap.MapsTo l v S -> NatMap.In l S.
+Proof.
+  intros.
+  apply NatMapFacts.find_mapsto_iff in H.
+  apply NatMapFacts.in_find_iff. unfold not. intros.
+  rewrite H0 in H. discriminate.
+Qed.
+
+
+Lemma StringMap_mapsto_in: forall (t : Type) (m : StringMap.t t) k e,
+  StringMap.MapsTo k e m -> StringMap.In k m.
+Proof.
+  intros.
+  apply StringMapFacts.find_mapsto_iff in H.
+  apply StringMapFacts.in_find_iff. unfold not. intros.
+  rewrite H0 in H. discriminate.
+Qed.
+
+
+Lemma NatMap_add_unique_then_restrict_no_change : forall (S : store) l v,
+  ~ NatMap.In l S ->
+  NatMap.Equal S (NatMapProperties.restrict (NatMapProperties.update S ( NatMap.add l v (NatMap.empty Z))) S).
+Proof.
+  intros. rewrite NatMapFacts.Equal_mapsto_iff.
+  split.
+  - intros. apply NatMapProperties.restrict_mapsto_iff. split.
+    + apply NatMapProperties.update_mapsto_iff. right. split.
+      * assumption.
+      * apply NatMapFacts.not_find_in_iff in H as HfindlinS.
+        unfold not. rewrite NatMapFacts.add_in_iff. intros.
+        destruct H1.
+        -- apply NatMapFacts.find_mapsto_iff in H0 as HfindkinS.
+           rewrite <- H1 in HfindkinS. rewrite HfindkinS in HfindlinS. discriminate.
+        -- apply NatMapFacts.empty_in_iff in H1. apply H1.
+    + apply NatMap_mapsto_in in H0. assumption.
+  - intros. apply NatMapProperties.restrict_mapsto_iff in H0.
+    destruct H0. apply NatMapProperties.update_mapsto_iff in H0.
+    destruct H0.
+    + apply NatMapFacts.add_mapsto_iff in H0.
+      * destruct H0.
+        -- destruct H0. rewrite <- H0 in H1. contradiction.
+        -- destruct H0. apply NatMapFacts.empty_mapsto_iff in H2. destruct H2.
+    + destruct H0. assumption.
+Qed.
+
+
+Theorem NatMap_disjoint_diff_Equal : forall (S1 : store) (S2 : store),
+  NatMapProperties.Disjoint S1 S2 ->
+  NatMap.Equal S1 (NatMapProperties.diff (NatMapProperties.update S1 S2) S2).
+Proof.
+  intros. apply NatMapFacts.Equal_mapsto_iff. intros. split.
+  - intros. apply NatMapProperties.diff_mapsto_iff. split.
+    + apply NatMapProperties.update_mapsto_iff. right. split.
+      * assumption.
+      * unfold NatMapProperties.Disjoint in H.
+        apply NatMap_mapsto_in in H0. unfold not. intros. unfold not in H.
+        apply H with k. split.
+        -- assumption.
+        -- assumption.
+    + unfold NatMapProperties.Disjoint in H.
+      apply NatMap_mapsto_in in H0. unfold not. intros. unfold not in H.
+      apply H with k. split.
+      * assumption.
+      * assumption.
+  - intros. apply NatMapProperties.diff_mapsto_iff in H0. destruct H0.
+    apply NatMapProperties.update_mapsto_iff in H0. destruct H0.
+    * apply NatMap_mapsto_in in H0. contradiction.
+    * destruct H0. apply H0.
+Qed.
+
+
+Theorem NatMap_disjoint_restrict_Equal : forall (S1 : store) (S2 : store),
+  NatMapProperties.Disjoint S1 S2 ->
+  NatMap.Equal S1 (NatMapProperties.restrict (NatMapProperties.update S1 S2) S1).
+Proof.
+  intros.
+  apply NatMapFacts.Equal_mapsto_iff. intros. split.
+  - intros. apply NatMapProperties.restrict_mapsto_iff. split.
+    + apply NatMapProperties.update_mapsto_iff. right. split.
+      * assumption.
+      * unfold NatMapProperties.Disjoint in H.
+        apply NatMap_mapsto_in in H0. unfold not. intros. unfold not in H.
+        apply H with k. split.
+        -- assumption.
+        -- assumption.
+    + apply NatMap_mapsto_in in H0. assumption.
+  - rewrite NatMapProperties.restrict_mapsto_iff.
+    rewrite NatMapProperties.update_mapsto_iff.
+    intros. destruct H0. destruct H0.
+    + exfalso. unfold NatMapProperties.Disjoint in H. unfold not in H.
+      apply H with k. split.
+      * assumption.
+      * apply NatMap_mapsto_in in H0. assumption.
+    + destruct H0. assumption.
+Qed.
