proof_of_soundness/Theorems.v
@@ -8,162 +8,23 @@
 
 Require Import
   Coq.FSets.FMapList
+  Coq.Logic.Classical_Prop
   Coq.Lists.List
   Coq.Strings.String
-  ZArith.
+  Coq.ZArith.ZArith.
 
 From Cpp2C Require Import
   Syntax
   ConfigVars
+  MapTheorems
   EvalRules
   Transformations.
-
-
-Lemma NatMap_Empty_empty : forall (t : Type) (m : NatMap.t t),
-  NatMap.Empty (elt:=_) m ->
-  NatMap.Equal m (NatMap.empty _).
-Proof.
-  intros.
-  unfold NatMap.Empty in H.
-  apply NatMapProperties.elements_Empty in H.
-  unfold NatMap.Equal. intros.
-  rewrite NatMapFacts.elements_o. rewrite H. simpl.
-  rewrite NatMapFacts.empty_o. reflexivity.
-Qed.
-
-
-Lemma StringMap_Empty_empty : forall (t : Type) (m : StringMap.t t),
-  StringMap.Empty (elt:=_) m ->
-  StringMap.Equal m (StringMap.empty _).
-Proof.
-  intros.
-  unfold StringMap.Empty in H.
-  apply StringMapProperties.elements_Empty in H.
-  unfold StringMap.Equal. intros.
-  rewrite StringMapFacts.elements_o. rewrite H. simpl.
-  rewrite StringMapFacts.empty_o. reflexivity.
-Qed.
-
-
-Lemma NatMap_restrict_refl: forall (S : store),
-  NatMap.Equal S (NatMapProperties.restrict S S).
-Proof.
-  intros. rewrite NatMapFacts.Equal_mapsto_iff.
-  intros. rewrite NatMapProperties.restrict_mapsto_iff.
-  split; intros.
-  - (* -> *)
-    split.
-    + apply H.
-    + apply NatMapFacts.find_mapsto_iff in H.
-      apply NatMapFacts.in_find_iff. unfold not.
-      intros. rewrite H0 in H. discriminate H.
-  - (* <- *)
-    apply H.
-Qed.
-
-
-Lemma NatMap_mapsto_in: forall (S : store) l v,
-  NatMap.MapsTo l v S -> NatMap.In l S.
-Proof.
-  intros.
-  apply NatMapFacts.find_mapsto_iff in H.
-  apply NatMapFacts.in_find_iff. unfold not. intros.
-  rewrite H0 in H. discriminate.
-Qed.
-
-
-Lemma StringMap_mapsto_in: forall (t : Type) (m : StringMap.t t) k e,
-  StringMap.MapsTo k e m -> StringMap.In k m.
-Proof.
-  intros.
-  apply StringMapFacts.find_mapsto_iff in H.
-  apply StringMapFacts.in_find_iff. unfold not. intros.
-  rewrite H0 in H. discriminate.
-Qed.
-
-
-Lemma NatMap_add_unique_then_restrict_no_change : forall (S : store) l v,
-  ~ NatMap.In l S ->
-  NatMap.Equal S (NatMapProperties.restrict (NatMapProperties.update S ( NatMap.add l v (NatMap.empty Z))) S).
-Proof.
-  intros. rewrite NatMapFacts.Equal_mapsto_iff.
-  split.
-  - intros. apply NatMapProperties.restrict_mapsto_iff. split.
-    + apply NatMapProperties.update_mapsto_iff. right. split.
-      * assumption.
-      * apply NatMapFacts.not_find_in_iff in H as HfindlinS.
-        unfold not. rewrite NatMapFacts.add_in_iff. intros.
-        destruct H1.
-        -- apply NatMapFacts.find_mapsto_iff in H0 as HfindkinS.
-           rewrite <- H1 in HfindkinS. rewrite HfindkinS in HfindlinS. discriminate.
-        -- apply NatMapFacts.empty_in_iff in H1. apply H1.
-    + apply NatMap_mapsto_in in H0. assumption.
-  - intros. apply NatMapProperties.restrict_mapsto_iff in H0.
-    destruct H0. apply NatMapProperties.update_mapsto_iff in H0.
-    destruct H0.
-    + apply NatMapFacts.add_mapsto_iff in H0.
-      * destruct H0.
-        -- destruct H0. rewrite <- H0 in H1. contradiction.
-        -- destruct H0. apply NatMapFacts.empty_mapsto_iff in H2. destruct H2.
-    + destruct H0. assumption.
-Qed.
-
-
-Theorem NatMap_disjoint_diff_Equal : forall (S1 : store) (S2 : store),
-  NatMapProperties.Disjoint S1 S2 ->
-  NatMap.Equal S1 (NatMapProperties.diff (NatMapProperties.update S1 S2) S2).
-Proof.
-  intros. apply NatMapFacts.Equal_mapsto_iff. intros. split.
-  - intros. apply NatMapProperties.diff_mapsto_iff. split.
-    + apply NatMapProperties.update_mapsto_iff. right. split.
-      * assumption.
-      * unfold NatMapProperties.Disjoint in H.
-        apply NatMap_mapsto_in in H0. unfold not. intros. unfold not in H.
-        apply H with k. split.
-        -- assumption.
-        -- assumption.
-    + unfold NatMapProperties.Disjoint in H.
-      apply NatMap_mapsto_in in H0. unfold not. intros. unfold not in H.
-      apply H with k. split.
-      * assumption.
-      * assumption.
-  - intros. apply NatMapProperties.diff_mapsto_iff in H0. destruct H0.
-    apply NatMapProperties.update_mapsto_iff in H0. destruct H0.
-    * apply NatMap_mapsto_in in H0. contradiction.
-    * destruct H0. apply H0.
-Qed.
-
-
-Theorem NatMap_disjoint_restrict_Equal : forall (S1 : store) (S2 : store),
-  NatMapProperties.Disjoint S1 S2 ->
-  NatMap.Equal S1 (NatMapProperties.restrict (NatMapProperties.update S1 S2) S1).
-Proof.
-  intros.
-  apply NatMapFacts.Equal_mapsto_iff. intros. split.
-  - intros. apply NatMapProperties.restrict_mapsto_iff. split.
-    + apply NatMapProperties.update_mapsto_iff. right. split.
-      * assumption.
-      * unfold NatMapProperties.Disjoint in H.
-        apply NatMap_mapsto_in in H0. unfold not. intros. unfold not in H.
-        apply H with k. split.
-        -- assumption.
-        -- assumption.
-    + apply NatMap_mapsto_in in H0. assumption.
-  - rewrite NatMapProperties.restrict_mapsto_iff.
-    rewrite NatMapProperties.update_mapsto_iff.
-    intros. destruct H0. destruct H0.
-    + exfalso. unfold NatMapProperties.Disjoint in H. unfold not in H.
-      apply H with k. split.
-      * assumption.
-      * apply NatMap_mapsto_in in H0. assumption.
-    + destruct H0. assumption.
-Qed.
 
 
 Lemma no_side_effects_no_store_change : forall e,
   ~ ExprHasSideEffects e ->
   forall S E G F M v S',
-  ExprEval S E G F M e v S' ->
+  EvalExpr S E G F M e v S' ->
   NatMap.Equal S S'.
 Proof.
   intros e H S E G F M v S' E1.
@@ -174,7 +35,7 @@ Proof.
   - apply IHE1. apply H.
   - apply IHE1. apply H.
   - unfold ExprHasSideEffects in H. fold ExprHasSideEffects in H.
-    apply demorgan in H.
+    apply Classical_Prop.not_or_and in H.
     rewrite <- IHE1_1 in IHE1_2.
     apply IHE1_2.  apply H. apply H.
   - unfold ExprHasSideEffects in H. contradiction.
@@ -187,7 +48,7 @@ Qed.
 Lemma no_side_effects_no_store_change_eq : forall e,
   ~ ExprHasSideEffects e ->
   forall S E G F M v S',
-  ExprEval S E G F M e v S' ->
+  EvalExpr S E G F M e v S' ->
   S = S'.
 Proof.
   intros e H S E G F M v S' E1.
@@ -198,7 +59,7 @@ Proof.
   - apply IHE1. apply H.
   - apply IHE1. apply H.
   - unfold ExprHasSideEffects in H. fold ExprHasSideEffects in H.
-    apply demorgan in H.
+    apply Classical_Prop.not_or_and in H.
     rewrite <- IHE1_1 in IHE1_2.
     apply IHE1_2.  apply H. apply H.
   - unfold ExprHasSideEffects in H. contradiction.
@@ -208,11 +69,11 @@ Proof.
 Qed.
 
 
-Lemma no_side_effects_expreval_expreval : forall e,
+Lemma no_side_effects_evalexpr_evalexpr : forall e,
   ~ ExprHasSideEffects e ->
   forall S E G F M v S',
-  ExprEval S E G F M e v S' ->
-  ExprEval S E G F M e v S.
+  EvalExpr S E G F M e v S' ->
+  EvalExpr S E G F M e v S.
 Proof.
   intros e H S E G F M v S' E1.
   induction E1.
@@ -222,7 +83,7 @@ Proof.
   - apply E_ParenExpr. apply IHE1. assumption.
   - apply E_UnExpr. apply IHE1. assumption.
   - unfold ExprHasSideEffects in H. fold ExprHasSideEffects in H.
-    apply demorgan in H. destruct H. apply E_BinExpr with S'.
+    apply Classical_Prop.not_or_and in H. destruct H. apply E_BinExpr with S'.
     + assumption.
     + apply no_side_effects_no_store_change_eq in E1_1.
       * subst. apply IHE1_2. assumption.
@@ -274,7 +135,7 @@ Qed.
 
 
 Lemma skip_no_side_effects : forall S E G F M S',
-  StmtEval S E G F M Skip S' ->
+  EvalStmt S E G F M Skip S' ->
   NatMap.Equal S S'.
 Proof.
   intros. induction H. reflexivity.
@@ -286,16 +147,16 @@ Qed.
    Coq's built-in induction tactic is not powerful enough to provide
    us with the induction hypotheses necessary to prove these lemmas, so
    we must define our own induction schema for these proofs *)
-Scheme ExprEval_mut := Induction for ExprEval Sort Prop
-with StmtEval_mut := Induction for StmtEval Sort Prop
+Scheme EvalExpr_mut := Induction for EvalExpr Sort Prop
+with EvalStmt_mut := Induction for EvalStmt Sort Prop
 with EvalArgs_mut := Induction for EvalArgs Sort Prop.
 
 
-Lemma stmteval_notin_F_add_stmteval : forall S E G F M stmt S',
-  StmtEval S E G F M stmt S' ->
+Lemma evalstmt_notin_F_add_evalstmt : forall S E G F M stmt S',
+  EvalStmt S E G F M stmt S' ->
   forall x fdef,
     ~ StringMap.In x F ->
-    StmtEval S E G (StringMap.add x fdef F) M stmt S'.
+    EvalStmt S E G (StringMap.add x fdef F) M stmt S'.
 Proof.
 (*
   This proof could be solved instead with the following ltac code:
@@ -304,36 +165,45 @@ Proof.
   as a simple demonstration of how to use schemas *)
   intros. apply (
     (* First we apply the appropriate schema like a tactic *)
-    StmtEval_mut
+    EvalStmt_mut
       (* Then we have to define a custom inductive hypothesis for each Prop
          that the one we are inducting over is mutually inductive with
-         (in this case just the StmtEval Prop since statement evaluation
+         (in this case just the EvalStmt Prop since statement evaluation
          currently only includes skip statements, which don't
          involve expressions) *)
-      (fun S E G F M stmt S' (h : StmtEval S E G F M stmt S') =>
-        StmtEval S E G (StringMap.add x fdef F) M stmt S')
+      (fun S E G F M stmt S' (h : EvalStmt S E G F M stmt S') =>
+        EvalStmt S E G (StringMap.add x fdef F) M stmt S')
   ); try constructor; auto.
 Qed.
 
 
-Lemma expreval_notin_F_add_expreval : forall S E G F M e v S',
-  ExprEval S E G F M e v S' ->
+Lemma evalstmt_disjoint_update_F_evalstmt : forall S E G F M stmt S',
+  EvalStmt S E G F M stmt S' ->
+  forall F',
+    StringMapProperties.Disjoint F F' ->
+    EvalStmt S E G (StringMapProperties.update F F') M stmt S'.
+Proof.
+  intros. induction H; try constructor. Qed.
+
+
+Lemma evalexpr_notin_F_add_evalexpr : forall S E G F M e v S',
+  EvalExpr S E G F M e v S' ->
   forall x fdef,
     ~ StringMap.In x F ->
-    ExprEval S E G (StringMap.add x fdef F) M e v S'.
+    EvalExpr S E G (StringMap.add x fdef F) M e v S'.
 Proof.
   apply (
-    ExprEval_mut
-      (* ExprEval *)
-      (fun S E G F M e v S' (h : ExprEval S E G F M e v S' ) =>
+    EvalExpr_mut
+      (* EvalExpr *)
+      (fun S E G F M e v S' (h : EvalExpr S E G F M e v S' ) =>
         forall x fdef,
         ~ StringMap.In x F ->
-        ExprEval S E G (StringMap.add x fdef F) M e v S' )
-      (* StmtEval *)
-      (fun S E G F M stmt S' (h : StmtEval S E G F M stmt S' ) =>
+        EvalExpr S E G (StringMap.add x fdef F) M e v S' )
+      (* EvalStmt *)
+      (fun S E G F M stmt S' (h : EvalStmt S E G F M stmt S' ) =>
         forall x fdef,
         ~ StringMap.In x F ->
-        StmtEval S E G (StringMap.add x fdef F) M stmt S' )
+        EvalStmt S E G (StringMap.add x fdef F) M stmt S' )
       (* EvalArgs *)
       (fun Sprev Ecaller G F M es vs Snext (h : EvalArgs Sprev Ecaller G F M es vs Snext) =>
         forall x fdef,
@@ -346,7 +216,7 @@ Proof.
   - apply E_Assign_Local with l S'; auto.
   - apply E_Assign_Global with l S'; auto.
   - apply E_FunctionCall with
-      params fstmt fexpr ls Sargs S' S'' S''' Ef S'''' vs; auto.
+      params fstmt fexpr ls Ef Sargs S' S'' S''' S'''' vs; auto.
     + apply StringMapFacts.add_mapsto_iff. right. split.
       * unfold not; intros. subst. apply StringMap_mapsto_in in m.
         contradiction.
@@ -356,7 +226,134 @@ Proof.
 Qed.
 
 
+Lemma evalexpr_disjoint_update_F_evalexpr : forall S E G F M e v S',
+  EvalExpr S E G F M e v S' ->
+  forall F',
+    StringMapProperties.Disjoint F F' ->
+    EvalExpr S E G (StringMapProperties.update F F') M e v S'.
+Proof.
+  apply (
+    EvalExpr_mut
+      (* EvalExpr *)
+      (fun S E G F M e v S' (h : EvalExpr S E G F M e v S' ) =>
+        forall F',
+          StringMapProperties.Disjoint F F' ->
+          EvalExpr S E G (StringMapProperties.update F F') M e v S' )
+      (* EvalStmt *)
+      (fun S E G F M stmt S' (h : EvalStmt S E G F M stmt S' ) =>
+        forall F',
+          StringMapProperties.Disjoint F F' ->
+          EvalStmt S E G (StringMapProperties.update F F') M stmt S' )
+      (* EvalArgs *)
+      (fun Sprev Ecaller G F M es vs Snext (h : EvalArgs Sprev Ecaller G F M es vs Snext) =>
+        forall F',
+          StringMapProperties.Disjoint F F' ->
+          EvalArgs Sprev Ecaller G (StringMapProperties.update F F') M es vs Snext)
+    ); intros; try constructor; auto.
+  - apply E_LocalVar with l; auto.
+  - apply E_GlobalVar with l; auto.
+  - apply E_BinExpr with S'; auto.
+  - apply E_Assign_Local with l S'; auto.
+  - apply E_Assign_Global with l S'; auto.
+  - apply E_FunctionCall with
+      params fstmt fexpr ls Ef Sargs S' S'' S''' S'''' vs; auto.
+    + apply StringMapProperties.update_mapsto_iff. right. split.
+      * auto.
+      * apply StringMap_mapsto_in in m.
+        unfold StringMapProperties.Disjoint in H2.
+        assert (~ (StringMap.In (elt:=function_definition) x F /\
+                    StringMap.In (elt:=function_definition) x F')).
+        { apply H2. }
+        apply Classical_Prop.not_and_or in H3. destruct H3.
+        -- contradiction.
+        -- auto.
+  - apply E_MacroInvocation with params mexpr M' MP ef; auto.
+  - apply EvalArgs_cons with Snext; auto.
+Qed.
 
+
+Lemma evalargs_notin_F_add_evalargs : forall S E G F M es vs S',
+  EvalArgs S E G F M es vs S' ->
+  forall x fdef,
+    ~ StringMap.In x F ->
+    EvalArgs S E G (StringMap.add x fdef F) M es vs S'.
+Proof.
+  apply (
+    EvalArgs_mut
+      (* EvalExpr *)
+      (fun S E G F M e v S' (h : EvalExpr S E G F M e v S' ) =>
+        forall x fdef,
+        ~ StringMap.In x F ->
+        EvalExpr S E G (StringMap.add x fdef F) M e v S' )
+      (* EvalStmt *)
+      (fun S E G F M stmt S' (h : EvalStmt S E G F M stmt S' ) =>
+        forall x fdef,
+        ~ StringMap.In x F ->
+        EvalStmt S E G (StringMap.add x fdef F) M stmt S' )
+      (* EvalArgs *)
+      (fun Sprev Ecaller G F M es vs Snext (h : EvalArgs Sprev Ecaller G F M es vs Snext) =>
+        forall x fdef,
+        ~ StringMap.In x F ->
+        EvalArgs Sprev Ecaller G (StringMap.add x fdef F) M es vs Snext)
+    ); intros; try constructor; auto.
+  - apply E_LocalVar with l; auto.
+  - apply E_GlobalVar with l; auto.
+  - apply E_BinExpr with S'; auto.
+  - apply E_Assign_Local with l S'; auto.
+  - apply E_Assign_Global with l S'; auto.
+  - apply E_FunctionCall with params fstmt fexpr ls Ef Sargs S' S'' S''' S'''' vs; auto.
+    + apply StringMapFacts.add_mapsto_iff. right. split.
+      * unfold not; intros. subst. apply StringMap_mapsto_in in m.
+        contradiction.
+      * auto.
+  - apply E_MacroInvocation with params mexpr M' MP ef; auto.
+  - apply EvalArgs_cons with Snext; auto.
+Qed.
+
+
+Lemma evalargs_disjoint_update_F_evalargs : forall S E G F M es vs S',
+  EvalArgs S E G F M es vs S' ->
+  forall F',
+    StringMapProperties.Disjoint F F' ->
+    EvalArgs S E G (StringMapProperties.update F F') M es vs S'.
+Proof.
+  apply (
+    EvalArgs_mut
+      (* EvalExpr *)
+      (fun S E G F M e v S' (h : EvalExpr S E G F M e v S' ) =>
+        forall F',
+          StringMapProperties.Disjoint F F' ->
+          EvalExpr S E G (StringMapProperties.update F F') M e v S' )
+      (* EvalStmt *)
+      (fun S E G F M stmt S' (h : EvalStmt S E G F M stmt S' ) =>
+        forall F',
+          StringMapProperties.Disjoint F F' ->
+          EvalStmt S E G (StringMapProperties.update F F') M stmt S' )
+      (* EvalArgs *)
+      (fun Sprev Ecaller G F M es vs Snext (h : EvalArgs Sprev Ecaller G F M es vs Snext) =>
+        forall F',
+          StringMapProperties.Disjoint F F' ->
+          EvalArgs Sprev Ecaller G (StringMapProperties.update F F') M es vs Snext)
+    ); intros; try constructor; auto.
+  - apply E_LocalVar with l; auto.
+  - apply E_GlobalVar with l; auto.
+  - apply E_BinExpr with S'; auto.
+  - apply E_Assign_Local with l S'; auto.
+  - apply E_Assign_Global with l S'; auto.
+  - apply E_FunctionCall with params fstmt fexpr ls Ef Sargs S' S'' S''' S'''' vs; auto.
+    + apply StringMapProperties.update_mapsto_iff. right. split.
+      * auto.
+      * apply StringMap_mapsto_in in m.
+        unfold StringMapProperties.Disjoint in H2.
+        assert (~ (StringMap.In (elt:=function_definition) x F /\
+                    StringMap.In (elt:=function_definition) x F')).
+        { apply H2. }
+        apply Classical_Prop.not_and_or in H3. destruct H3.
+        -- contradiction.
+        -- auto.
+  - apply E_MacroInvocation with params mexpr M' MP ef; auto.
+  - apply EvalArgs_cons with Snext; auto.
+Qed.
 
 
 Theorem side_effect_free_function_no_side_effects :
@@ -374,10 +371,10 @@ Theorem side_effect_free_function_no_side_effects :
   NatMap.Equal Sargs (NatMapProperties.of_list (combine ls vs)) ->
   NatMapProperties.Disjoint S' Sargs ->
   NatMap.Equal S'' (NatMapProperties.update S' Sargs) ->
-  StmtEval S'' Ef G F M fstmt S''' ->
-  ExprEval S''' Ef G F M fexpr v S'''' ->
+  EvalStmt S'' Ef G F M fstmt S''' ->
+  EvalExpr S''' Ef G F M fexpr v S'''' ->
   NatMap.Equal S''''' (NatMapProperties.restrict S'''' S) ->
-  ExprEval S E G F M (CallOrInvocation x es) v S''''' ->
+  EvalExpr S E G F M (CallOrInvocation x es) v S''''' ->
   NatMap.Equal S''''' S.
 Proof.
   intros. subst. apply no_side_effects_no_store_change_arg_eval in H5.
@@ -420,8 +417,8 @@ Proof.
       apply forall_es_combine_forall_snd with (ks:=params) (es:=es).
       assumption. rewrite H1 in Hfind. apply Hfind.
     + auto.
-  - simpl in *. apply demorgan in H. destruct H.
-    apply demorgan. split.
+  - simpl in *. apply Classical_Prop.not_or_and in H. destruct H.
+    apply Classical_Prop.and_not_or. split.
     + apply IHmexpr1. assumption.
     + apply IHmexpr2. assumption.
   - simpl in H. contradiction.
@@ -437,8 +434,8 @@ Theorem side_effect_free_macro_no_side_effects :
   Forall (fun e => ~ExprHasSideEffects e) es ->
   MP = combine params es ->
   ef = msub MP mexpr ->
-  ExprEval S E G F M' ef v S' ->
-  ExprEval S E G F M (CallOrInvocation x es) v S' ->
+  EvalExpr S E G F M' ef v S' ->
+  EvalExpr S E G F M (CallOrInvocation x es) v S' ->
   NatMap.Equal S S'.
 Proof.
   intros.
@@ -462,8 +459,8 @@ Example transform_side_effect_free_macro_sound :
   Forall (fun e => ~ExprHasSideEffects e) es ->
   MP = combine params es ->
   ef = msub MP mexpr ->
-  ExprEval S E G F M' ef v S0' ->
-  ExprEval S E G F M (CallOrInvocation x es) v S0' ->
+  EvalExpr S E G F M' ef v S0' ->
+  EvalExpr S E G F M (CallOrInvocation x es) v S0' ->
 
   Forall (fun e => ~ ExprHasSideEffects e) es ->
   ~ ExprHasSideEffects mexpr ->
@@ -484,13 +481,13 @@ Example transform_side_effect_free_macro_sound :
   (* Combine the argument store into the original store *)
   NatMap.Equal S'' (NatMapProperties.update S' Sargs) ->
   (* Evaluate the function's body *)
-  StmtEval S'' Ef G F' M Skip S''' ->
-  ExprEval S''' Ef G F' M mexpr v S'''' ->
+  EvalStmt S'' Ef G F' M Skip S''' ->
+  EvalExpr S''' Ef G F' M mexpr v S'''' ->
   (* Only keep in the store the L-value mappings that were there when
      the function was called; i.e., remove from the store all mappings
      whose L-value is in Ef/Sargs. *)
   NatMap.Equal S''''' (NatMapProperties.restrict S'''' S) ->
-  ExprEval S E G F' M (CallOrInvocation y es) v S''''' ->
+  EvalExpr S E G F' M (CallOrInvocation y es) v S''''' ->
   NatMap.Equal S0' S'''''.
 Proof.
   intros.
@@ -516,10 +513,10 @@ Qed.
 
 
 (* This proof is easy right now because we only have Skip statements *)
-Lemma stmteval_transformargs_stmteval : forall S E G F M stmt S' F' stmt',
-  StmtEval S E G F M stmt S' ->
+Lemma evalstmt_transformargs_evalstmt : forall S E G F M stmt S' F' stmt',
+  EvalStmt S E G F M stmt S' ->
   TransformStmt M F stmt F' stmt' ->
-  StmtEval S E G F' M stmt S'.
+  EvalStmt S E G F' M stmt S'.
 Proof.
   intros. induction H0. assumption.
 Qed.
@@ -530,107 +527,95 @@ with TransformArgs_mut := Induction for TransformArgs Sort Prop
 with TransformStmt_mut := Induction for TransformStmt Sort Prop.
 
 
-
-(* Attempt 1: Induction over the transformation with schema *)
-Theorem transform_expr_sound : forall M F e F' e',
+(* Attempt 2: Induction over the transformation with schema *)
+Theorem transform_expr_sound_mut : forall M F e F' e',
   TransformExpr M F e F' e' ->
   (* The proof will not work if these variables were introduced sooner.
      Doing so would interfere with the induction hypothesis *)
   forall S E G v S',
-    ExprEval S E G F M e v S' ->
-    ExprEval S E G F' M e' v S'.
+    EvalExpr S E G F M e v S' ->
+    EvalExpr S E G F' M e' v S'.
 Proof.
   intros M F e F' e' H. apply (TransformExpr_mut
     (* TransformExpr *)
     (fun M F e F' e' (h : TransformExpr M F e F' e') =>
     forall S E G v S',
-    ExprEval S E G F M e v S' ->
-    ExprEval S E G F' M e' v S')
+      EvalExpr S E G F M e v S' ->
+      EvalExpr S E G F' M e' v S')
     (* TransformArgs *)
     (fun M F es F' es' (h : TransformArgs M F es F' es') =>
-    forall S E G v S',
-    ExprEval S E G F M e v S' ->
-    ExprEval S E G F' M e' v S')
+    forall S Ecaller G vs S',
+      EvalArgs S Ecaller G F M es vs S' ->
+      EvalArgs S Ecaller G F' M es' vs S')
     (* TransformStmt *)
     (fun M F stmt F' stmt' (h : TransformStmt M F stmt F' stmt') =>
-    forall S E G v S',
-    ExprEval S E G F M e v S' ->
-    ExprEval S E G F' M e' v S')); auto.
+    forall S E G S',
+      EvalStmt S E G F M stmt S' ->
+      EvalStmt S E G F' M stmt' S')); auto.
   - intros. inversion_clear H1. apply E_ParenExpr. apply H0; auto.
   - intros. inversion_clear H1. apply E_UnExpr. apply H0; auto.
   - intros. inversion_clear H2. apply E_BinExpr with S'0.
-Abort.
-
-
-(* Attempt 2: Induction over the evaluation *)
-Theorem expreval_transform_expreval : forall S E G F M e v S',
-  ExprEval S E G F M e v S' ->
-  forall F' e',
-    TransformExpr M F e F' e' ->
-    ExprEval S E G F' M e' v S'.
-Proof.
-  intros S E G F M e v S' H. induction H; try (intros F' e' H; inversion_clear H; econstructor; auto).
-  - intros. inversion_clear H1. apply E_LocalVar with l; auto.
-  - intros. inversion_clear H2. apply E_GlobalVar with l; auto.
-  - intros. inversion_clear H0. apply E_ParenExpr; auto.
-  - intros. inversion_clear H0. apply E_UnExpr; auto.
-  - intros. inversion_clear H1. apply E_BinExpr with S'.
-    + apply IHExprEval1.
-Abort.
-
-
-(* Attempt 3: Induction over the evaluation with schema *)
-Theorem expreval_transform_expreval : forall S E G F M e v S',
-  ExprEval S E G F M e v S' ->
-  forall F' e',
-    TransformExpr M F e F' e' ->
-    ExprEval S E G F' M e' v S'.
-Proof.
-  intros S E G F M e v S' H.
-  apply (
-    ExprEval_mut
-      (* ExprEval *)
-      (fun S E G F M e v S' (h : ExprEval S E G F M e v S' ) =>
-        forall F' e',
-          TransformExpr M F e F' e' ->
-          ExprEval S E G F' M e' v S')
-      (* StmtEval *)
-      (fun S E G F M stmt S' (h : StmtEval S E G F M stmt S' ) =>
-        forall F' stmt',
-          TransformStmt M F stmt F' stmt' ->
-          StmtEval S E G F' M stmt' S')
-      (* EvalArgs *)
-      (fun Sprev Ecaller G F M es vs Snext (h : EvalArgs Sprev Ecaller G F M es vs Snext) =>
-        forall F' es',
-          TransformArgs M F es F' es' ->
-          EvalArgs Sprev Ecaller G F' M es' vs Snext)
-    ); try (intros; econstructor; auto).
-  - intros. inversion_clear H0. constructor.
-  - intros. inversion_clear H0. apply E_LocalVar with l; auto.
-  - intros. inversion_clear H0. apply E_GlobalVar with l; auto.
-  - intros. inversion_clear H1. apply E_ParenExpr; auto.
-  - intros. inversion_clear H1. apply E_UnExpr; auto.
-  - intros. inversion_clear H2. apply E_BinExpr with S'0.
-    + apply H5. apply H0. (* apply H3. *) admit.
-    + apply H1. apply H4.
-  - intros. inversion_clear H1. apply E_Assign_Local with l S'0; auto.
-  - intros. inversion_clear H1. apply E_Assign_Global with l S'0; auto.
+    + subst. apply evalexpr_disjoint_update_F_evalexpr; auto.
+    + subst. apply H1. apply evalexpr_disjoint_update_F_evalexpr. auto. auto.
+  - intros. inversion_clear H1.
+    + apply E_Assign_Local with l S'0; auto.
+    + apply E_Assign_Global with l S'0; auto.
   - intros. inversion_clear H3.
-    + apply H6 with
-          params0 fstmt0 fexpr0 params fstmt fexpr in H5. inversion H5. subst.
-      apply E_FunctionCall with
-        params fstmt' fexpr' ls Sargs S'0 S'' S''' Ef S'''' vs; auto.
-      * rewrite H10. apply StringMapFacts.add_mapsto_iff. left. auto.
-      * apply H0. admit.
-      * apply H1. admit.
-      * apply H2. admit.
+    + apply StringMapFacts.find_mapsto_iff in m.
+      apply StringMapFacts.find_mapsto_iff in H5.
+      rewrite H5 in *. inversion m. subst. clear m.
+      apply E_FunctionCall with params fstmt' fexpr' ls Ef Sargs S'0 S'' S''' S'''' vs; auto.
+      * apply StringMapFacts.add_mapsto_iff. left; auto.
+      * apply evalargs_notin_F_add_evalargs; auto.
+        apply evalargs_disjoint_update_F_evalargs; auto.
+        apply evalargs_disjoint_update_F_evalargs; auto.
+      * apply evalstmt_notin_F_add_evalstmt; auto.
+        apply evalstmt_disjoint_update_F_evalstmt; auto.
+        apply H1.
+        apply evalstmt_disjoint_update_F_evalstmt; auto.
+      * apply evalexpr_notin_F_add_evalexpr; auto.
+        apply H2.
+        apply evalexpr_disjoint_update_F_evalexpr; auto.
+        apply evalexpr_disjoint_update_F_evalexpr; auto.
     + apply StringMap_mapsto_in in H4. contradiction.
   - intros. inversion_clear H1.
     + apply StringMap_mapsto_in in m. contradiction.
-    + apply H3 with
-        params0 mexpr0 params mexpr in H2. inversion H2. subst.
+    + apply StringMapFacts.find_mapsto_iff in m.
+      apply StringMapFacts.find_mapsto_iff in H2.
+      rewrite H2 in *. inversion m. subst. clear m.
+      assert (
+        EvalArgs S E G F0 M0 es vs S' /\
+        StringMap.Equal Ef (StringMapProperties.of_list (combine params ls)) /\
+        NatMap.Equal Sargs (NatMapProperties.of_list (combine ls vs)) /\
+        NatMapProperties.Disjoint S' Sargs /\
+        NatMap.Equal S'' (NatMapProperties.update S' Sargs) /\
+        EvalStmt S'' Ef G F0 M0 Skip S''' /\
+        EvalExpr S''' Ef G F0 M0 mexpr v0 S'''' /\
+        NatMap.Equal S''''' (NatMapProperties.restrict S'''' S)
+     ). { apply a. }
+     destruct H1. destruct H3. destruct H5. destruct H6. destruct H8. destruct H9.
+     destruct H10.
       apply E_FunctionCall with
-        (params:=params) (fstmt:=Skip) (fexpr:=mexpr) (ls:=ls) (Sargs:=Sargs) (S':=S')
-        (S'':=S'') (S''':=S''') (Ef:=Ef) (S'''':=S'''') (vs:=vs); auto.
-      * rewrite H8. apply StringMapFacts.add_mapsto_iff. left; auto.
-      * Abort.
+        (params:=params) (fstmt:=Skip) (fexpr:=mexpr) (ls:=ls)
+        (Ef:=Ef) (Sargs:=Sargs) (S':=S') (S'':=S'') (S''':=S''') (S'''':=S'''')
+        (vs:=vs); auto.
+      * apply StringMapFacts.add_mapsto_iff. left; auto.
+      * apply evalargs_notin_F_add_evalargs; auto.
+      * apply evalstmt_notin_F_add_evalstmt; auto.
+        apply evalstmt_disjoint_update_F_evalstmt; auto.
+      * apply evalexpr_notin_F_add_evalexpr; auto.
+        apply evalexpr_disjoint_update_F_evalexpr; auto.
+      *
+        (* Here is where we prove that they evaluate to the same state *)
+        assert (~ ExprHasSideEffects (msub (combine params es) mexpr)).
+        { apply no_side_effects_msub_no_side_effects with params es; auto. }
+        apply no_side_effects_no_store_change in H7; auto.
+        apply no_side_effects_no_store_change_arg_eval in H1; auto.
+        apply skip_no_side_effects in H9; auto.
+        apply no_side_effects_no_store_change in H10; auto.
+        rewrite <- H7. rewrite <- H10. rewrite <- H9. rewrite H8. rewrite <- H1.
+        apply NatMap_disjoint_restrict_Equal. rewrite H1. auto.
+  - intros. inversion_clear H2. apply EvalArgs_cons with Snext.
+    + subst. apply evalexpr_disjoint_update_F_evalexpr; auto.
+    + subst. apply H1; auto using evalargs_disjoint_update_F_evalargs.
+Qed.
